\documentclass[11pt]{article}

\input{../../tex/defs.tex}

% Useful syntax commands
\newcommand{\jarr}[1]{\left[#1\right]}   % \jarr{x: y} = {x: y}
\newcommand{\jobj}[1]{\left\{#1\right\}} % \jobj{1, 2} = [1, 2]
\newcommand{\pgt}[1]{\, > {#1}}          % \pgt{1} = > 1
\newcommand{\plt}[1]{\, < {#1}}          % \plt{2} = < 2
\newcommand{\peq}[1]{\, = {#1}}          % \peq{3} = = 3
\newcommand{\prop}[1]{\langle{#1}\rangle}% \prop{x} = <x>
\newcommand{\matches}[2]{{#1}\sim{#2}}   % \matches{a}{b} = a ~ b
\newcommand{\aeps}{\varepsilon}          % \apes = epsilon
\newcommand{\akey}[2]{.{#1}\,{#2}}       % \akey{s}{a} = .s a
\newcommand{\aidx}[2]{[#1]\,{#2}}        % \aidx{i}{a} = [i] a
\newcommand{\apipe}[1]{\mid {#1}}        % \apipe{a} = | a

% Other useful syntax commands:
%
% \msf{x} = x (not italicised)
% \falset = false
% \truet = true
% \tnum = num
% \tbool = bool
% \tstr = str


\begin{document}

\hwtitle
{Assignment 1}
{Anyang He (heanyang1)} %% REPLACE THIS WITH YOUR NAME/ID

\problem{Problem 1}

Part 1:

\begin{alignat*}{1}
  \msf{Property}~p ::= \qamp \varepsilon                                       \\
  \mid \qamp >n \mid\ =n \mid\ <n                                              \\
  \mid \qamp =s                                                                \\
  \mid \qamp (p)                                                               \\
  \mid \qamp p_1 \vee p_2 \mid p_1 \wedge p_2                                  \\
  \\
  \msf{Schema}~\tau ::= \qamp \tnum \prop{p} \mid\ \tstr \prop{p} \mid\ \tbool \\
  % Lists can only have elements of a single schema, so there is no *
  \mid \qamp [\tau]                                                            \\
  \mid \qamp \{(s:\tau)^*\}                                                    \\
\end{alignat*}

Part 2:

% mathpar is the environment for writing inference rules. It takes care of
% the spacing and line breaks automatically. Use "\\" in the premises to
% space out multiple assumptions.
\begin{mathpar}

  \ir{S-Bool-False}{\ }{\matches{\falset}{\tbool}}

  \ir{S-Bool-True}{\ }{\matches{\truet}{\tbool}}

  % Inference rules go here
  \ir{S-String-Terminate}{\ }{\matches{s}{\tstr \prop{\varepsilon} } }

  \ir{S-Number-Terminate}{\ }{\matches{n}{\tnum \prop{\varepsilon} } }

  \ir{S-String-Equal}{s=s_0}{\matches{s}{\tstr \prop{=s_0}}}

  \ir{S-Number-Equal}{n=n_0}{\matches{n}{\tnum \prop{=n_0}}}

  \ir{S-Number-Greater}{n>n_0}{\matches{n}{\tnum \prop{>n_0}}}

  \ir{S-Number-Lesser}{n<n_0}{\matches{n}{\tnum \prop{<n_0}}}

  \ir{S-String-And}{\matches{s}{\tstr \prop{p_1}}\ \matches{s}{\tstr \prop{p_2}}}{\matches{s}{\tstr \prop{p_1\wedge p_2}}}

  % assume that \(p_1 \vee p_2 = p_2 \vee p_1\)
  \ir{S-String-Or}{\matches{s}{\tstr \prop{p_1}}}{\matches{s}{\tstr \prop{p_1\vee p_2}}}

  \ir{S-Number-And}{\matches{n}{\tnum \prop{p_1}}\ \matches{n}{\tnum \prop{p_2}}}{\matches{n}{\tnum \prop{p_1\wedge p_2}}}

  \ir{S-Number-Or}{\matches{n}{\tnum \prop{p_1}}}{\matches{n}{\tnum \prop{p_1\vee p_2}}}

  \ir{S-List}{\matches{\forall i=0 \dots |j| - 1.\ j_i}{\tau} }{\matches{[j^*]}{[\tau]} }

  \ir{S-Dict}{\matches{\forall s'\in s.\ j_{s'} }{\tau_{s'} } }{\matches{ \{(s:j)^*\} }{ \{(s:\tau)^*\} } }
\end{mathpar}

\problem{Problem 2}

Part 1:

\begin{mathpar}
  % Inference rules go here

  % I use val to represent terminate state here
  \ir{A-Terminate}{ }{ (\varepsilon,j) \val{} }

  \ir{A-Dict}{j=\{s':j', \ldots\}}{\steps{ (.sa,j) }{ (a,j') } }

  \ir{A-Index}{j=[\dots,j_n,\dots] }{\steps{ ([n]a,j) }{ (a',j_n) } }

  \ir{A-Map-Empty}{ }{\steps{(|\varepsilon,j)}{(\varepsilon,j)}}

  \ir{A-Map}{\forall n = 0 \ldots |j| - 1. \ \steps{(a,j_n)}{(a',j'_n)} }{\steps{ (|a,j) }{ (|a',[\dots,j'_n,\dots]) } }
\end{mathpar}

Part 2:

\begin{mathpar}
  % Inference rules go here
  \ir{V-Terminate}{\ }{\matches{\varepsilon}{\tau} }

  \ir{V-Dict}{\matches{a}{\tau} }{\matches{.sa}{ \{s:\tau,\dots\} } }

  \ir{V-Index}{\matches{a}{\tau} }{\matches{[n]a}{[\tau]} }

  \ir{V-Map}{\matches{a}{\tau} }{\matches{|a}{[\tau]} }
\end{mathpar}

I made a stronger claim here so that the V-Map part can be proved clearly. The idea is that any object with the same type can be accessed in the same way.

\textit{(Strong) Accessor safety}: for all \(a, \tau\) such that \(\matches{a}{\tau}\), there exists accessors \(a_1, a_2, \ldots, a_k\) such that \(a_1 = a, a_k = \varepsilon\) and for all \(\matches{j}{\tau}\), then there exists objects \(j_1, j_2, \ldots, j_k\) such that \(j_1=j\),
\begin{equation}\label{eq_steps}
  \steps{(a_1,j_1)}{}\steps{(a_2,j_2)}{}\ldots\steps{}{(a_k,j_k)}.
\end{equation}

\begin{proof}
  \
  % Proof goes here.
  \begin{enumerate}
    \item If \(a=\varepsilon\), by V-Terminate, for all \(\tau\), \(\matches{a}{\tau}\).

          For every \(j\), define \(a_1=a=\varepsilon, j_1=j\). Because \((a,j)=(a_1,j_1)=(\varepsilon,j_1)\), therefore the theorem holds for \(a=\varepsilon\).
    \item Suppose that \(a=.s'a'\), \(\matches{a'}{\tau'}\), there exists accessors \(a_1, a_2, \ldots, a_k\) such that \(a_1 = a', a_k = \varepsilon\) and for all \(\matches{j}{\tau'}\), there exists objects \(j_1, j_2, \ldots, j_k\) such that \(j_1=j\) and equation (\ref{eq_steps}) holds.

          By V-Dict, \(\matches{a}{ \{s':\tau',\dots\} }\) (which means \(\matches{a}{\{(s:\tau)^*\}}\) such that \(s' \in s\) and \(\tau_{s'}=\tau'\)).

          For all \(\matches{j}{ \{s':\tau',\dots\} }\), by inversion lemma and S-Dict, \(j=\{(s:j)^*\}\) and \(\matches{j_{s'}}{\tau_{s'}}=\tau'\).

          Because \(\matches{j_{s'}}{\tau'}\), by inductive hypothesis, there exists objects \(j_{s'}^{(1)},j_{s'}^{(2)},\ldots,j_{s'}^{(k)}\) such that \(j_{s'}=j_{s'}^{(1)}\),
          \[\steps{(a_1,j_{s'}^{(1)})}{}\steps{(a_2,j_{s'}^{(2)})}{}\ldots\steps{}{(a_k,j_{s'}^{(k)})}.\]

          Because \(j=\{(s:j)^*\}\), \(s'\in s\), by A-Dict, \(\steps{(a,j)}{(a',j_{s'})}=(a_1,j_{s'}^{(1)})\).
          
          Therefore the theorem holds for \(a=.s'a'\) where \(a, a_1, a_2, \ldots, a_k\) described above is the set of accessors that satisfies the condition.
    \item Suppose that \(a=[n]a'\), \(\matches{a'}{\tau'}\), and for all \(\matches{j}{\tau'}\), there exists accessors \(a_1, a_2, \ldots, a_k\) such that \(a_1 = a', a_k = \varepsilon\) and for all \(\matches{j}{\tau'}\), then there exists objects \(j_1, j_2, \ldots, j_k\) such that \(j_1=j\) and equation (\ref{eq_steps}) holds.

          By V-Index, \(\matches{a}{[\tau']}\).

          For all \(\matches{j}{[\tau']}\), by inversion lemma and S-List, \(j=[\dots,j_n,\dots]\) and \(\matches{j_n}{\tau'}\).

          By inductive hypothesis, there exists objects \(j_{n}^{(1)},j_{n}^{(2)},\ldots,j_{n}^{(k)}\) such that \(j_{n}=j_{n}^{(1)}\),
          \[\steps{(a_1,j_{n}^{(1)})}{}\steps{(a_2,j_{n}^{(2)})}{}\ldots\steps{}{(a_k,j_{n}^{(k)})}.\]

          Because \(j=[\dots,j_n,\dots]\), by A-Index, \(\steps{(a,j)}{(a',j_n)}=(a_1,j_n^{(1)})\).

          Therefore the theorem holds for \(a=[n]a'\) where \(a, a_1, a_2, \ldots, a_k\) described above is the set of accessors that satisfies the condition.
    
    \item If \(a=|\varepsilon\), by V-Terminate, for every \(\tau\), \(\matches{\varepsilon}{\tau}\).
    
          By V-Map, for every \(\tau\), \(a=\matches{|\varepsilon}{[\tau]}\).
    
          By A-Map-Empty, for every \(\tau\), for every \(j\) such that \(\matches{j}{[\tau]}\), \((a,j)=\steps{(|\varepsilon,j)}{(\varepsilon,j)}\).
    
          Therefore the theorem holds for \(a=|e\).

    \item Suppose that \(a=|a'\), \(\matches{a'}{\tau'}\), there exists accessors \(a_1, a_2, \ldots, a_k\) such that \(a_1 = a', a_k = \varepsilon\) and for all \(\matches{j}{\tau'}\), then there exists objects \(j_1, j_2, \ldots, j_k\) such that \(j_1=j\) and equation (\ref{eq_steps}) holds.
    
          We claim that \(|a_1, |a_2, \ldots, |a_k, \varepsilon\) is the accessors that makes the theorem hold for \(a=|a'\).

          By V-Map, \(\matches{a}{[\tau']}\). For every \(\matches{j}{[\tau']}\), we need to find the objects \(j^{(1)},j^{(2)},\ldots,j^{(k+1)}\) such that
          \begin{equation}\label{eq_map}
            (a,j)=\steps{(|a_1,j^{(1)})}{}\steps{(|a_2,j^{(2)})}{}\ldots\steps{}{(|a_k,j^{(k)})}\steps{}{(\varepsilon,j^{(k+1)})}.
          \end{equation}

          By inductive hypothesis, for all \(n\), there exists objects \(j_{n}^{(1)},j_{n}^{(2)},\ldots,j_{n}^{(k)}\) such that \(j_{n}=j_{n}^{(1)}\),
          \[\steps{(a_1,j_{n}^{(1)})}{}\steps{(a_2,j_{n}^{(2)})}{}\ldots\steps{}{(a_k,j_{n}^{(k)})}.\]

          Let
          \[j^{(1)}=[\ldots,j_n^{(1)},\ldots],\quad j^{(2)}=[\ldots,j_n^{(2)},\ldots],\quad\ldots\quad j^{(k)}=j^{(k+1)}=[\ldots,j_n^{(k)},\ldots],\]
          then by A-Map, \(\steps{(a_i,j_{n}^{(i)})}{(a_{i+1},j_{n}^{(i+1)})}\) implies \(\steps{(|a_i,j^{(i)})}{(|a_{i+1},j^{(i+1)})}\). Therefore
          \[\steps{(|a_1,j^{(1)})}{}\steps{(|a_2,j^{(2)})}{}\ldots\steps{}{(|a_k,j^{(k)})}.\]

          Because \(a_k=\varepsilon\), by A-Map-Empty, \(\steps{(|a_k,j^{(k)})}{(\varepsilon,j^{(k)})}=(\varepsilon,j^{(k+1)})\).

          Because \(j_{n}=j_{n}^{(1)}\), therefore \(j=[\ldots,j_n,\ldots]=[\ldots,j_n^{(1)},\ldots]=j^{(1)}\). Therefore the \(j^{(i)}\) satisfies equation (\ref{eq_map}).\qedhere
  \end{enumerate}
\end{proof}

\end{document}
